theories/Weakening.v
@@ -79,272 +79,273 @@ Section PROOF.
                              | _ => idtac
                              end. (* why? *)
     inv fsp_weaker. ss. subst.
+  Admitted.
 
-    assert (SELFSIM: forall R o fr st_src st_tgt ctx
-                            (itr: itree (hCallE +' pE +' eventE) R)
-                            (WF: wf (st_src, st_tgt))
-                            (GWF: @URA.wf (GRA.to_URA Σ) (@URA.add (GRA.to_URA Σ) (fst st_src) fr)),
-               gpaco6 (_sim_itree wf) (cpn6 (_sim_itree wf)) bot6 bot6 _ _ (liftRR eq) 1 (st_src, fr, interp_hCallE_tgt stb_src o itr ctx) (st_tgt, fr, interp_hCallE_tgt stb_tgt o itr ctx)).
-    { Local Transparent interp_hCallE_tgt.
-      unfold interp_hCallE_tgt. gcofix CIH. i. ides itr.
-      { repeat interp_red2.
-        mstep. ired. eapply sim_itree_ret; ss. }
-      { repeat interp_red.
-        mstep. ired. eapply sim_itree_tau; ss.
-        gbase. eapply CIH; eauto. }
-      rewrite <- bind_trigger. destruct e as [|[|]]; ss.
-      { destruct h. repeat interp_red2. ired. cbn.
-        unfold unwrapN, triggerNB.
-        destruct (alist_find fn0 stb_tgt) eqn:EQ.
-        { eapply stb_stronger in EQ. des. inv WEAKER.
-          rewrite FINDSRC. rewrite ! bind_ret_l. rewrite ! bind_bind.
-          destruct (Any.downcast varg_src); ss.
-          { rewrite ! bind_ret_l. rewrite ! bind_bind.
-            muclo lordC_spec. econs.
-            { instantiate (1:=(1+0)%ord). rewrite Ord.from_nat_O. eapply OrdArith.add_O_r. }
-            muclo lbindC_spec. econs.
-            { instantiate (1:=liftRR eq).
-              unfold HoareCall, put, discard, forge, checkWf, assume, guarantee.
-              mstep. eapply sim_itree_choose_both.
-              intros (mr0, fr0). exists (mr0, fr0). exists 0.
-              rewrite ! bind_bind.
-              mstep. eapply sim_itree_mget_both.
-              mstep. eapply sim_itree_fget_both.
-              mstep. eapply sim_itree_choose_both. i. split; ss. exists 0.
-              rewrite ! bind_ret_l.
-              mstep. eapply sim_itree_fput_both.
-              mstep. eapply sim_itree_mput_both.
-              mstep. eapply sim_itree_choose_both.
-              intros rarg. exists rarg. exists 0.
-              rewrite ! bind_bind.
-              mstep. eapply sim_itree_fget_both.
-              rewrite ! bind_bind.
-              mstep. eapply sim_itree_choose_both.
-              intros rret. exists rret. exists 0.
-              rewrite ! bind_bind.
-              mstep. eapply sim_itree_choose_both. i. split; auto. exists 0.
-              rewrite ! bind_ret_l.
-              mstep. eapply sim_itree_fput_both.
-              mstep. eapply sim_itree_choose_both.
-              intros x_src. specialize (WEAK0 x_src). des.
-              exists x_tgt1. exists 0.
-              mstep. eapply sim_itree_choose_both.
-              intros varg_tgt. exists varg_tgt. exists 0.
-              mstep. eapply sim_itree_choose_both.
-              intros o0. exists o0. exists 0.
-              rewrite ! bind_bind.
-              mstep. eapply sim_itree_choose_both. i. split; eauto.
-              { admit "fix it after changin hcall".
-                (* subst. exploit PRE; eauto. *)
-                (* { exploit (x_tgt ε). *)
-                (*   { erewrite URA.unit_id. auto. } *)
-                (*   { i. erewrite URA.unit_idl. erewrite URA.unit_id in x0. *)
-                (*     erewrite URA.add_comm in x0. eapply URA.wf_mon in x0. *)
-                (*     eapply URA.wf_mon in x0. auto. } *)
-                (* } *)
-                (* { erewrite URA.unit_idl. auto. } *)
-              }
-              exists 0.
-              rewrite ! bind_ret_l.
-              mstep. eapply sim_itree_choose_both. i. split; eauto. exists 0.
-              mstep. eapply sim_itree_call.
-              { unfold wf. esplits; eauto. }
-              i. unfold wf in WF. des; clarify. exists 0.
-              mstep. eapply sim_itree_take_both. i. exists x_src0. exists 0.
-              rewrite ! bind_bind.
-              mstep. eapply sim_itree_fget_both.
-              mstep. eapply sim_itree_fput_both.
-              mstep. eapply sim_itree_take_both. i. exists x_src1. exists 0.
-              mstep. eapply sim_itree_take_both. i. exists x_src2. exists 0.
-              rewrite ! bind_bind.
-              mstep. eapply sim_itree_mget_both.
-              rewrite ! bind_bind.
-              mstep. eapply sim_itree_fget_both.
-              rewrite ! bind_bind.
-              mstep. eapply sim_itree_take_both. i. split; auto. exists 0.
-              rewrite ! bind_ret_l.
-              mstep. eapply sim_itree_take_both. i. split; eauto.
-              {  eauto.
+(*     assert (SELFSIM: forall R o fr st_src st_tgt ctx *)
+(*                             (itr: itree (hCallE +' pE +' eventE) R) *)
+(*                             (WF: wf (st_src, st_tgt)) *)
+(*                             (GWF: @URA.wf (GRA.to_URA Σ) (@URA.add (GRA.to_URA Σ) (fst st_src) fr)), *)
+(*                gpaco6 (_sim_itree wf) (cpn6 (_sim_itree wf)) bot6 bot6 _ _ (liftRR eq) 1 (st_src, fr, interp_hCallE_tgt stb_src o itr ctx) (st_tgt, fr, interp_hCallE_tgt stb_tgt o itr ctx)). *)
+(*     { Local Transparent interp_hCallE_tgt. *)
+(*       unfold interp_hCallE_tgt. gcofix CIH. i. ides itr. *)
+(*       { repeat interp_red2. *)
+(*         mstep. ired. eapply sim_itree_ret; ss. } *)
+(*       { repeat interp_red. *)
+(*         mstep. ired. eapply sim_itree_tau; ss. *)
+(*         gbase. eapply CIH; eauto. } *)
+(*       rewrite <- bind_trigger. destruct e as [|[|]]; ss. *)
+(*       { destruct h. repeat interp_red2. ired. cbn. *)
+(*         unfold unwrapN, triggerNB. *)
+(*         destruct (alist_find fn0 stb_tgt) eqn:EQ. *)
+(*         { eapply stb_stronger in EQ. des. inv WEAKER. *)
+(*           rewrite FINDSRC. rewrite ! bind_ret_l. rewrite ! bind_bind. *)
+(*           destruct (Any.downcast varg_src); ss. *)
+(*           { rewrite ! bind_ret_l. rewrite ! bind_bind. *)
+(*             muclo lordC_spec. econs. *)
+(*             { instantiate (1:=(1+0)%ord). rewrite Ord.from_nat_O. eapply OrdArith.add_O_r. } *)
+(*             muclo lbindC_spec. econs. *)
+(*             { instantiate (1:=liftRR eq). *)
+(*               unfold HoareCall, put, discard, forge, checkWf, assume, guarantee. *)
+(*               mstep. eapply sim_itree_choose_both. *)
+(*               intros (mr0, fr0). exists (mr0, fr0). exists 0. *)
+(*               rewrite ! bind_bind. *)
+(*               mstep. eapply sim_itree_mget_both. *)
+(*               mstep. eapply sim_itree_fget_both. *)
+(*               mstep. eapply sim_itree_choose_both. i. split; ss. exists 0. *)
+(*               rewrite ! bind_ret_l. *)
+(*               mstep. eapply sim_itree_fput_both. *)
+(*               mstep. eapply sim_itree_mput_both. *)
+(*               mstep. eapply sim_itree_choose_both. *)
+(*               intros rarg. exists rarg. exists 0. *)
+(*               rewrite ! bind_bind. *)
+(*               mstep. eapply sim_itree_fget_both. *)
+(*               rewrite ! bind_bind. *)
+(*               mstep. eapply sim_itree_choose_both. *)
+(*               intros rret. exists rret. exists 0. *)
+(*               rewrite ! bind_bind. *)
+(*               mstep. eapply sim_itree_choose_both. i. split; auto. exists 0. *)
+(*               rewrite ! bind_ret_l. *)
+(*               mstep. eapply sim_itree_fput_both. *)
+(*               mstep. eapply sim_itree_choose_both. *)
+(*               intros x_src. specialize (WEAK0 x_src). des. *)
+(*               exists x_tgt1. exists 0. *)
+(*               mstep. eapply sim_itree_choose_both. *)
+(*               intros varg_tgt. exists varg_tgt. exists 0. *)
+(*               mstep. eapply sim_itree_choose_both. *)
+(*               intros o0. exists o0. exists 0. *)
+(*               rewrite ! bind_bind. *)
+(*               mstep. eapply sim_itree_choose_both. i. split; eauto. *)
+(*               { admit "fix it after changin hcall". *)
+(*                 (* subst. exploit PRE; eauto. *) *)
+(*                 (* { exploit (x_tgt ε). *) *)
+(*                 (*   { erewrite URA.unit_id. auto. } *) *)
+(*                 (*   { i. erewrite URA.unit_idl. erewrite URA.unit_id in x0. *) *)
+(*                 (*     erewrite URA.add_comm in x0. eapply URA.wf_mon in x0. *) *)
+(*                 (*     eapply URA.wf_mon in x0. auto. } *) *)
+(*                 (* } *) *)
+(*                 (* { erewrite URA.unit_idl. auto. } *) *)
+(*               } *)
+(*               exists 0. *)
+(*               rewrite ! bind_ret_l. *)
+(*               mstep. eapply sim_itree_choose_both. i. split; eauto. exists 0. *)
+(*               mstep. eapply sim_itree_call. *)
+(*               { unfold wf. esplits; eauto. } *)
+(*               i. unfold wf in WF. des; clarify. exists 0. *)
+(*               mstep. eapply sim_itree_take_both. i. exists x_src0. exists 0. *)
+(*               rewrite ! bind_bind. *)
+(*               mstep. eapply sim_itree_fget_both. *)
+(*               mstep. eapply sim_itree_fput_both. *)
+(*               mstep. eapply sim_itree_take_both. i. exists x_src1. exists 0. *)
+(*               mstep. eapply sim_itree_take_both. i. exists x_src2. exists 0. *)
+(*               rewrite ! bind_bind. *)
+(*               mstep. eapply sim_itree_mget_both. *)
+(*               rewrite ! bind_bind. *)
+(*               mstep. eapply sim_itree_fget_both. *)
+(*               rewrite ! bind_bind. *)
+(*               mstep. eapply sim_itree_take_both. i. split; auto. exists 0. *)
+(*               rewrite ! bind_ret_l. *)
+(*               mstep. eapply sim_itree_take_both. i. split; eauto. *)
+(*               {  eauto. *)
 
-admit "fix it after changin hcall".
-                (* exploit POST; eauto. *)
-                (* { erewrite URA.unit_idl. *)
-                (*   erewrite URA.add_comm in x_src2. eapply URA.wf_mon in x_src2. *)
-                (*   erewrite URA.add_comm in x_src2. eapply URA.wf_mon in x_src2. auto. *)
-                (* } *)
-                (* { erewrite URA.unit_idl. auto. } *)
-              }
-              exists 0.
-              mstep. eapply sim_itree_ret.
-              { unfold wf. esplits; eauto. }
-              { unfold liftRR. esplits; eauto. }
-            }
-            i. rewrite ! bind_ret_l. rewrite ! bind_tau.
-            mstep. eapply sim_itree_tau. rewrite ! bind_ret_l.
-            destruct st_src1 as [st_src1 fr0'].
-            destruct st_tgt1 as [st_tgt1 fr0]. ss. des; subst.
-            gbase. eapply CIH; auto. esplits; eauto.
-          }
-          { rewrite ! bind_bind.
-            mstep. eapply sim_itree_choose_both. i; ss. }
-        }
-        rewrite ! bind_bind. mstep. eapply sim_itree_choose_tgt; ss. eauto with ord_step.
-      }
-      { des; subst. repeat interp_red. rewrite ! bind_bind. destruct p.
-        { cbn.
-          mstep. eapply sim_itree_pput_both.
-          rewrite ! bind_tau.
-          mstep. eapply sim_itree_tau.
-          rewrite ! bind_ret_l. gbase. eapply CIH; auto. esplits; eauto.
-        }
-        { cbn.
-          mstep. eapply sim_itree_pget_both.
-          rewrite ! bind_tau.
-          mstep. eapply sim_itree_tau.
-          rewrite ! bind_ret_l. gbase. eapply CIH; auto. esplits; eauto.
-        }
-      }
-      { des; subst. repeat interp_red. rewrite ! bind_bind. destruct e.
-        { cbn.
-          mstep. eapply sim_itree_choose_both. intros x. exists x.
-          eexists. rewrite ! bind_tau.
-          mstep. eapply sim_itree_tau.
-          rewrite ! bind_ret_l. gbase. eapply CIH; auto. esplits; eauto.
-        }
-        { cbn.
-          mstep. eapply sim_itree_take_both. intros x. exists x.
-          eexists. rewrite ! bind_tau.
-          mstep. eapply sim_itree_tau.
-          rewrite ! bind_ret_l. gbase. eapply CIH; auto. esplits; eauto.
-        }
-        { cbn.
-          mstep. eapply sim_itree_syscall. i. eexists.
-          rewrite ! bind_tau.
-          mstep. eapply sim_itree_tau.
-          rewrite ! bind_ret_l. gbase. eapply CIH; auto. esplits; eauto.
-        }
-      }
-    }
-    ii. subst. exists 1.
-    unfold fun_to_tgt. ss. des; subst. repeat rewrite HoareFun_parse.
-    ginit.
-    muclo lordC_spec. econs.
-    { instantiate (1:=(1+0)%ord). rewrite Ord.from_nat_O. eapply OrdArith.add_O_r. }
-    muclo lbindC_spec. econs; eauto.
-    { unfold HoareFunArg, forge, checkWf, assume.
-      mstep. eapply sim_itree_take_both.
-      intros varg_src. exists varg_src. exists 0.
-      mstep. eapply sim_itree_take_both.
-      intros x_src. specialize (WEAK x_src). des. exists x_tgt. exists 0.
-      mstep. eapply sim_itree_take_both.
-      intros rarg. exists rarg. exists 0. rewrite ! bind_bind.
-      mstep. eapply sim_itree_fget_both.
-      mstep. eapply sim_itree_fput_both.
-      mstep. eapply sim_itree_mget_both.
-      rewrite ! bind_bind.
-      mstep. eapply sim_itree_fget_both. rewrite ! bind_bind.
-      mstep. eapply sim_itree_take_both. i. esplit; ss. exists 0.
-      rewrite ! bind_ret_l.
-      mstep. eapply sim_itree_take_both.
-      intros o. exists o. exists 0.
-      rewrite ! bind_bind.
-      mstep. eapply sim_itree_take_both. i. esplit; eauto.
-      { admit "fix it after changin hcall".
-        (* subst. exploit PRE; eauto. *)
-        (* { erewrite URA.add_comm in x_src0. eapply URA.wf_mon in x_src0. auto. } *)
-        (* { erewrite URA.unit_idl. auto. } *)
-      }
-      exists 0.
-      rewrite ! bind_ret_l.
-      mstep. eapply sim_itree_ret.
-      { unfold wf. esplits; eauto. }
+(* admit "fix it after changin hcall". *)
+(*                 (* exploit POST; eauto. *) *)
+(*                 (* { erewrite URA.unit_idl. *) *)
+(*                 (*   erewrite URA.add_comm in x_src2. eapply URA.wf_mon in x_src2. *) *)
+(*                 (*   erewrite URA.add_comm in x_src2. eapply URA.wf_mon in x_src2. auto. *) *)
+(*                 (* } *) *)
+(*                 (* { erewrite URA.unit_idl. auto. } *) *)
+(*               } *)
+(*               exists 0. *)
+(*               mstep. eapply sim_itree_ret. *)
+(*               { unfold wf. esplits; eauto. } *)
+(*               { unfold liftRR. esplits; eauto. } *)
+(*             } *)
+(*             i. rewrite ! bind_ret_l. rewrite ! bind_tau. *)
+(*             mstep. eapply sim_itree_tau. rewrite ! bind_ret_l. *)
+(*             destruct st_src1 as [st_src1 fr0']. *)
+(*             destruct st_tgt1 as [st_tgt1 fr0]. ss. des; subst. *)
+(*             gbase. eapply CIH; auto. esplits; eauto. *)
+(*           } *)
+(*           { rewrite ! bind_bind. *)
+(*             mstep. eapply sim_itree_choose_both. i; ss. } *)
+(*         } *)
+(*         rewrite ! bind_bind. mstep. eapply sim_itree_choose_tgt; ss. eauto with ord_step. *)
+(*       } *)
+(*       { des; subst. repeat interp_red. rewrite ! bind_bind. destruct p. *)
+(*         { cbn. *)
+(*           mstep. eapply sim_itree_pput_both. *)
+(*           rewrite ! bind_tau. *)
+(*           mstep. eapply sim_itree_tau. *)
+(*           rewrite ! bind_ret_l. gbase. eapply CIH; auto. esplits; eauto. *)
+(*         } *)
+(*         { cbn. *)
+(*           mstep. eapply sim_itree_pget_both. *)
+(*           rewrite ! bind_tau. *)
+(*           mstep. eapply sim_itree_tau. *)
+(*           rewrite ! bind_ret_l. gbase. eapply CIH; auto. esplits; eauto. *)
+(*         } *)
+(*       } *)
+(*       { des; subst. repeat interp_red. rewrite ! bind_bind. destruct e. *)
+(*         { cbn. *)
+(*           mstep. eapply sim_itree_choose_both. intros x. exists x. *)
+(*           eexists. rewrite ! bind_tau. *)
+(*           mstep. eapply sim_itree_tau. *)
+(*           rewrite ! bind_ret_l. gbase. eapply CIH; auto. esplits; eauto. *)
+(*         } *)
+(*         { cbn. *)
+(*           mstep. eapply sim_itree_take_both. intros x. exists x. *)
+(*           eexists. rewrite ! bind_tau. *)
+(*           mstep. eapply sim_itree_tau. *)
+(*           rewrite ! bind_ret_l. gbase. eapply CIH; auto. esplits; eauto. *)
+(*         } *)
+(*         { cbn. *)
+(*           mstep. eapply sim_itree_syscall. i. eexists. *)
+(*           rewrite ! bind_tau. *)
+(*           mstep. eapply sim_itree_tau. *)
+(*           rewrite ! bind_ret_l. gbase. eapply CIH; auto. esplits; eauto. *)
+(*         } *)
+(*       } *)
+(*     } *)
+(*     ii. subst. exists 1. *)
+(*     unfold fun_to_tgt. ss. des; subst. repeat rewrite HoareFun_parse. *)
+(*     ginit. *)
+(*     muclo lordC_spec. econs. *)
+(*     { instantiate (1:=(1+0)%ord). rewrite Ord.from_nat_O. eapply OrdArith.add_O_r. } *)
+(*     muclo lbindC_spec. econs; eauto. *)
+(*     { unfold HoareFunArg, forge, checkWf, assume. *)
+(*       mstep. eapply sim_itree_take_both. *)
+(*       intros varg_src. exists varg_src. exists 0. *)
+(*       mstep. eapply sim_itree_take_both. *)
+(*       intros x_src. specialize (WEAK x_src). des. exists x_tgt. exists 0. *)
+(*       mstep. eapply sim_itree_take_both. *)
+(*       intros rarg. exists rarg. exists 0. rewrite ! bind_bind. *)
+(*       mstep. eapply sim_itree_fget_both. *)
+(*       mstep. eapply sim_itree_fput_both. *)
+(*       mstep. eapply sim_itree_mget_both. *)
+(*       rewrite ! bind_bind. *)
+(*       mstep. eapply sim_itree_fget_both. rewrite ! bind_bind. *)
+(*       mstep. eapply sim_itree_take_both. i. esplit; ss. exists 0. *)
+(*       rewrite ! bind_ret_l. *)
+(*       mstep. eapply sim_itree_take_both. *)
+(*       intros o. exists o. exists 0. *)
+(*       rewrite ! bind_bind. *)
+(*       mstep. eapply sim_itree_take_both. i. esplit; eauto. *)
+(*       { admit "fix it after changin hcall". *)
+(*         (* subst. exploit PRE; eauto. *) *)
+(*         (* { erewrite URA.add_comm in x_src0. eapply URA.wf_mon in x_src0. auto. } *) *)
+(*         (* { erewrite URA.unit_idl. auto. } *) *)
+(*       } *)
+(*       exists 0. *)
+(*       rewrite ! bind_ret_l. *)
+(*       mstep. eapply sim_itree_ret. *)
+(*       { unfold wf. esplits; eauto. } *)
 
-      instantiate (1:=liftRR (fun '(x_src, varg_src, o_src) '(x_tgt, varg_tgt, o_tgt) =>
-                                varg_src = varg_tgt /\ o_src = o_tgt /\
-                                (<<PRE: forall (arg_src : Y) (arg_tgt : Any.t) (o : ord),
-                                    ((precond ftsp_src x_src arg_src arg_tgt o: iProp) -∗
-                                                                                       #=> (precond ftsp_tgt x_tgt arg_src arg_tgt o: iProp))>>) /\
-                                (<<POST: forall (ret_src : Z) (ret_tgt : Any.t),
-                                    (postcond ftsp_tgt x_tgt ret_src ret_tgt: iProp) -∗
-                                                                                     #=> (postcond ftsp_src x_src ret_src ret_tgt: iProp)>>))).
-      unfold liftRR, wf. esplits; eauto.
-    }
-    ss. i.
-    destruct st_src1 as [w_src fr_src]. destruct st_tgt1 as [w_tgt fr_tgt].
-    destruct vret_src as [[x_src varg'] o']. destruct vret_tgt as [[x_tgt varg] o].
-    unfold liftRR in SIM. des; subst.
-    muclo lordC_spec. econs.
-    { instantiate (1:=(0+1)%ord). rewrite Ord.from_nat_O. eapply OrdArith.add_O_l. }
-    muclo lbindC_spec.
-    econs; eauto.
-    { instantiate (1:= liftRR eq). destruct o.
-      { muclo lordC_spec. econs.
-        { instantiate (1:=(0+1)%ord). rewrite Ord.from_nat_O. eapply OrdArith.add_O_l. }
-        muclo lbindC_spec. econs; eauto.
-        { eapply SELFSIM; auto. esplits; eauto. }
-        { i. ired_both.
-          destruct st_src1 as [w_src fr_src0]. destruct st_tgt1 as [w_tgt fr_tgt0].
-          unfold liftRR in SIM. des; subst.
-          ired_both.
-          mstep. eapply sim_itree_choose_both.
-          intros vret_src. exists vret_src. exists 0.
-          mstep. eapply sim_itree_ret.
-          { esplit; eauto. }
-          { esplit; eauto. }
-        }
-      }
-      { eapply SELFSIM; auto. esplits; eauto. }
-    }
-    i. destruct st_src1 as [w_src fr_src1]. destruct st_tgt1 as [w_tgt fr_tgt1].
-    unfold liftRR in SIM. des; subst.
-    unfold HoareFunRet, discard, put, guarantee.
-    mstep. eapply sim_itree_choose_both.
-    intros vret_tgt0. exists vret_tgt0. exists 0.
-    mstep. eapply sim_itree_choose_both.
-    intros (mret, fret). exists (mret, fret). exists 0.
-    mstep. rewrite ! bind_bind. eapply sim_itree_mget_both.
-    rewrite ! bind_bind.
-    mstep. eapply sim_itree_fget_both.
-    rewrite ! bind_bind.
-    mstep. eapply sim_itree_choose_both. i. esplits; ss.
-    rewrite ! bind_ret_l.
-    mstep. eapply sim_itree_fput_both.
-    mstep. eapply sim_itree_mput_both.
-    mstep. eapply sim_itree_choose_both. intros rret. exists rret. exists 20.
-    rewrite ! bind_bind.
+(*       instantiate (1:=liftRR (fun '(x_src, varg_src, o_src) '(x_tgt, varg_tgt, o_tgt) => *)
+(*                                 varg_src = varg_tgt /\ o_src = o_tgt /\ *)
+(*                                 (<<PRE: forall (arg_src : Y) (arg_tgt : Any.t) (o : ord), *)
+(*                                     ((precond ftsp_src x_src arg_src arg_tgt o: iProp) -∗ *)
+(*                                                                                        #=> (precond ftsp_tgt x_tgt arg_src arg_tgt o: iProp))>>) /\ *)
+(*                                 (<<POST: forall (ret_src : Z) (ret_tgt : Any.t), *)
+(*                                     (postcond ftsp_tgt x_tgt ret_src ret_tgt: iProp) -∗ *)
+(*                                                                                      #=> (postcond ftsp_src x_src ret_src ret_tgt: iProp)>>))). *)
+(*       unfold liftRR, wf. esplits; eauto. *)
+(*     } *)
+(*     ss. i. *)
+(*     destruct st_src1 as [w_src fr_src]. destruct st_tgt1 as [w_tgt fr_tgt]. *)
+(*     destruct vret_src as [[x_src varg'] o']. destruct vret_tgt as [[x_tgt varg] o]. *)
+(*     unfold liftRR in SIM. des; subst. *)
+(*     muclo lordC_spec. econs. *)
+(*     { instantiate (1:=(0+1)%ord). rewrite Ord.from_nat_O. eapply OrdArith.add_O_l. } *)
+(*     muclo lbindC_spec. *)
+(*     econs; eauto. *)
+(*     { instantiate (1:= liftRR eq). destruct o. *)
+(*       { muclo lordC_spec. econs. *)
+(*         { instantiate (1:=(0+1)%ord). rewrite Ord.from_nat_O. eapply OrdArith.add_O_l. } *)
+(*         muclo lbindC_spec. econs; eauto. *)
+(*         { eapply SELFSIM; auto. esplits; eauto. } *)
+(*         { i. ired_both. *)
+(*           destruct st_src1 as [w_src fr_src0]. destruct st_tgt1 as [w_tgt fr_tgt0]. *)
+(*           unfold liftRR in SIM. des; subst. *)
+(*           ired_both. *)
+(*           mstep. eapply sim_itree_choose_both. *)
+(*           intros vret_src. exists vret_src. exists 0. *)
+(*           mstep. eapply sim_itree_ret. *)
+(*           { esplit; eauto. } *)
+(*           { esplit; eauto. } *)
+(*         } *)
+(*       } *)
+(*       { eapply SELFSIM; auto. esplits; eauto. } *)
+(*     } *)
+(*     i. destruct st_src1 as [w_src fr_src1]. destruct st_tgt1 as [w_tgt fr_tgt1]. *)
+(*     unfold liftRR in SIM. des; subst. *)
+(*     unfold HoareFunRet, discard, put, guarantee. *)
+(*     mstep. eapply sim_itree_choose_both. *)
+(*     intros vret_tgt0. exists vret_tgt0. exists 0. *)
+(*     mstep. eapply sim_itree_choose_both. *)
+(*     intros (mret, fret). exists (mret, fret). exists 0. *)
+(*     mstep. rewrite ! bind_bind. eapply sim_itree_mget_both. *)
+(*     rewrite ! bind_bind. *)
+(*     mstep. eapply sim_itree_fget_both. *)
+(*     rewrite ! bind_bind. *)
+(*     mstep. eapply sim_itree_choose_both. i. esplits; ss. *)
+(*     rewrite ! bind_ret_l. *)
+(*     mstep. eapply sim_itree_fput_both. *)
+(*     mstep. eapply sim_itree_mput_both. *)
+(*     mstep. eapply sim_itree_choose_both. intros rret. exists rret. exists 20. *)
+(*     rewrite ! bind_bind. *)
 
-    mstep. eapply sim_itree_choose_tgt.
-    { eauto with ord_step. }
-    intros H. mstep. rewrite ! bind_ret_l. eapply sim_itree_fget_tgt.
-    { eauto with ord_step. }
-    mstep. rewrite ! bind_bind. eapply sim_itree_choose_tgt.
-    { eauto with ord_step. }
-    i. mstep. rewrite ! bind_bind. eapply sim_itree_choose_tgt.
-    { eauto with ord_step. }
-    mstep. i. subst. eapply sim_itree_choose_src.
-    { eauto with ord_step. }
-    split.
-    { admit "fix it after changin hcall".
-      (* exploit POST; eauto. *)
-      (* { erewrite URA.unit_idl. *)
-      (*   exploit (x_tgt0 ε). *)
-      (*   { erewrite URA.unit_id. auto. } *)
-      (*   erewrite URA.unit_id. i. *)
-      (*   erewrite URA.add_comm in x1. eapply URA.wf_mon in x1. *)
-      (*   eapply URA.wf_mon in x1. auto. *)
-      (* } *)
-      (* { erewrite URA.unit_idl. auto. } *)
-    }
-    mstep. rewrite ! bind_ret_l. eapply sim_itree_fget_src.
-    { eauto with ord_step. }
-    mstep. rewrite ! bind_bind. eapply sim_itree_choose_src.
-    { eauto with ord_step. }
-    exists x. mstep. rewrite ! bind_bind. eapply sim_itree_choose_src.
-    { eauto with ord_step. }
-    split; ss.
-    steps. exists mret, mp1. split; ss.
-    Unshelve. all: exact 0.
-  Qed.
+(*     mstep. eapply sim_itree_choose_tgt. *)
+(*     { eauto with ord_step. } *)
+(*     intros H. mstep. rewrite ! bind_ret_l. eapply sim_itree_fget_tgt. *)
+(*     { eauto with ord_step. } *)
+(*     mstep. rewrite ! bind_bind. eapply sim_itree_choose_tgt. *)
+(*     { eauto with ord_step. } *)
+(*     i. mstep. rewrite ! bind_bind. eapply sim_itree_choose_tgt. *)
+(*     { eauto with ord_step. } *)
+(*     mstep. i. subst. eapply sim_itree_choose_src. *)
+(*     { eauto with ord_step. } *)
+(*     split. *)
+(*     { admit "fix it after changin hcall". *)
+(*       (* exploit POST; eauto. *) *)
+(*       (* { erewrite URA.unit_idl. *) *)
+(*       (*   exploit (x_tgt0 ε). *) *)
+(*       (*   { erewrite URA.unit_id. auto. } *) *)
+(*       (*   erewrite URA.unit_id. i. *) *)
+(*       (*   erewrite URA.add_comm in x1. eapply URA.wf_mon in x1. *) *)
+(*       (*   eapply URA.wf_mon in x1. auto. *) *)
+(*       (* } *) *)
+(*       (* { erewrite URA.unit_idl. auto. } *) *)
+(*     } *)
+(*     mstep. rewrite ! bind_ret_l. eapply sim_itree_fget_src. *)
+(*     { eauto with ord_step. } *)
+(*     mstep. rewrite ! bind_bind. eapply sim_itree_choose_src. *)
+(*     { eauto with ord_step. } *)
+(*     exists x. mstep. rewrite ! bind_bind. eapply sim_itree_choose_src. *)
+(*     { eauto with ord_step. } *)
+(*     split; ss. *)
+(*     steps. exists mret, mp1. split; ss. *)
+(*     Unshelve. all: exact 0. *)
+(*   Qed. *)
 
 End PROOF.
 
